testdata/out/coq/event_proof_gk.v
@@ -20,16 +20,18 @@ Context `{!goGlobalsGS Σ}.
 Program Instance : IsPkgInit event_gk :=
   ltac2:(build_pkg_init ()).
 
-Definition has_encoding (encoded:list u8) (args:event_gk.Event.t) : Prop :=
+Definition has_encoding (encoded:list u8) (args:event_gk.S.t) : Prop :=
   ∃ (startTime_enc endTime_enc : list u8), 
-  encoded = (u32_le args.(event_gk.Event.id)) ++
-              (u64_le $ length $ args.(event_gk.Event.name')) ++ args.(event.Event.name') ++
+  encoded = (u32_le args.(event_gk.S.Id')) ++
+              (u64_le $ length $ args.(event_gk.S.Name')) ++ args.(event_gk.S.Name') ++
               startTime_enc ++
               endTime_enc
-  /\ TimeStamp_gk.has_encoding startTime_enc args.(startTime)
-  /\ TimeStamp_gk.has_encoding endTime_enc args.(endTime).
+  /\ length args.(event_gk.S.Name') < 2^64
+  /\ TimeStamp_gk.has_encoding startTime_enc args.(event_gk.S.StartTime')
+  /\ TimeStamp_gk.has_encoding endTime_enc args.(event_gk.S.EndTime').
 
-Lemma wp_Encode (args__c : event_gk.Event.t) (pre_sl : slice.t) (prefix : list u8) (dq : dfrac):
+Lemma wp_Encode (args__c : event_gk.S.t) (pre_sl : slice.t) (prefix : list u8) (dq : dfrac):
+  length args__c.(event_gk.S.Name') < 2^64 ->
   {{{
         is_pkg_init event_gk ∗
         own_slice pre_sl (DfracOwn 1) prefix ∗
@@ -44,48 +46,33 @@ Lemma wp_Encode (args__c : event_gk.Event.t) (pre_sl : slice.t) (prefix : list u
   }}}.
 
 Proof.
-  iIntros (?) "[Hown Hsl] HΦ".
-  wp_rec. wp_pures.
-  iUnfold own in "Hown". iNamed "Hown". rewrite Hown_struct.
-  wp_apply (wp_ref_to); first by val_ty.
-  iIntros (?) "Hptr". wp_pures.
+  intros Hnamelen.
+  wp_start as "[Hsl Hcap]". wp_auto.
 
-  wp_load. wp_apply (wp_WriteInt32 with "[$Hsl]").
-  iIntros (?) "Hsl". wp_store.
+  wp_apply (wp_WriteInt32 with "[$Hsl $Hcap]").
+  iIntros (?) "[Hsl Hcap]". wp_auto.
 
-  wp_apply wp_StringToBytes. iIntros (?) "Hargs_name_enc". wp_pures.
-  wp_apply (wp_slice_len).
-  iDestruct (own_slice_sz with "Hargs_name_enc") as "%Hargs_name_sz".
-  iApply own_slice_to_small in "Hargs_name_enc".
-  wp_load. wp_apply (wp_WriteInt with "[$Hsl]"). iIntros (?) "Hsl". wp_store.
-  wp_load. wp_apply (wp_WriteBytes with "[$Hsl $Hargs_name_enc]").
-  iIntros (?) "[Hsl _]". wp_store.
+  wp_apply wp_StringToBytes. iIntros (?) "HnameBytes". wp_auto.
+  wp_apply (wp_WriteLenPrefixedBytes with "[$Hsl $Hcap $HnameBytes]").
+  iIntros (?) "(Hsl & Hcap & HnameBytes)". wp_auto.
 
-  wp_load. wp_pures. wp_apply (TimeStamp.wp_Encode with "[$Hown_startTime $Hsl]").
-  iIntros (startTime_enc startTime_sl) "(%Hargs_startTime_enc & Hargs_startTime_own & Hsl)".
-  wp_store.
+  wp_apply (TimeStamp_gk.wp_Encode with "[$Hsl $Hcap]"); first trivial.
+  iIntros (startTime_enc ?) "(%Hargs_startTime_enc & Hsl & Hcap)". wp_auto.
 
-  wp_load. wp_pures. wp_apply (TimeStamp.wp_Encode with "[$Hown_endTime $Hsl]").
-  iIntros (endTime_enc endTime_sl) "(%Hargs_endTime_enc & Hargs_endTime_own & Hsl)".
-  wp_store.
+  wp_apply (TimeStamp_gk.wp_Encode with "[$Hsl $Hcap]"); first trivial.
+  iIntros (endTime_enc ?) "(%Hargs_endTime_enc & Hsl & Hcap)". wp_auto.
 
 
-  wp_load. iApply "HΦ". iModIntro. rewrite -?app_assoc.
+  iApply "HΦ". rewrite -?app_assoc.
   iFrame. iPureIntro.
 
-  unfold has_encoding. split.
-  {
+  unfold has_encoding. 
   exists startTime_enc, endTime_enc. 
-  rewrite ?string_bytes_length.
-  rewrite Hargs_name_sz.
   rewrite ?w64_to_nat_id.
-
   done.
-  
-  } done.
 Qed.
 
-Lemma wp_Decode (enc : list u8) (enc_sl : slice.t) (args__c : event_gk.Event.t) (suffix : list u8) (dq : dfrac):
+Lemma wp_Decode (enc : list u8) (enc_sl : slice.t) (args__c : event_gk.S.t) (suffix : list u8) (dq : dfrac):
   {{{
         is_pkg_init event_gk ∗
         ⌜ has_encoding enc args__c ⌝ ∗
@@ -93,33 +80,17 @@ Lemma wp_Decode (enc : list u8) (enc_sl : slice.t) (args__c : event_gk.Event.t) 
   }}}
     event_gk @ "Unmarshal" #enc_sl
   {{{
-        suff_sl, RET (#args__c, suff_sl);
+        suff_sl, RET (#args__c, #suff_sl);
         own_slice suff_sl dq suffix
   }}}.
 
 Proof.
-  iIntros (?) "[%Henc Hsl] HΦ". wp_rec.
-  wp_apply wp_ref_to; first done.
-  iIntros (l__s) "Hs". wp_pures.
-  
-  wp_apply wp_ref_of_zero; first done.
-  iIntros (l__id) "Hid". wp_pures.
-  
-  wp_apply wp_ref_of_zero; first done.
-  iIntros (l__name) "Hname". wp_pures.
-  
-  wp_apply wp_ref_of_zero; first done.
-  iIntros (l__startTime) "HstartTime". wp_pures.
-  
-  wp_apply wp_ref_of_zero; first done.
-  iIntros (l__endTime) "HendTime". wp_pures.
-  
+  wp_start as "[%Henc Hsl]". wp_auto.
   unfold has_encoding in Henc.
   destruct Henc as ( startTime_enc & endTime_enc & Henc & Henc_startTime & Henc_endTime ).
   rewrite Henc. rewrite -?app_assoc.
 
-  wp_load. wp_apply (wp_ReadInt32 with "[$Hsl]"). iIntros (?) "Hsl".
-  wp_pures. wp_store. wp_store.
+  wp_apply (wp_ReadInt32 with "[$Hsl]"). iIntros (?) "Hsl". wp_auto.
 
   wp_apply wp_ref_of_zero; first done. iIntros (nameLen) "HnameLen". wp_pures.
   wp_apply wp_ref_of_zero; first done. iIntros (nameBytes) "HnameBytes". wp_pures.
@@ -146,9 +117,13 @@ Proof.
   iDestruct (TimeStamp.own_val_ty with "Hown_endTime") as "%Hval_endTime".
   wp_pures. wp_store. wp_store.
 
-  wp_load. wp_load. wp_load. wp_load. wp_load.
-  wp_pures. iApply "HΦ". iModIntro. rewrite ?string_to_bytes_to_string. iFrame.
-  iPureIntro. reflexivity.
+  replace {|
+    event_gk.S.Id' := args__c.(event_gk.S.Id');
+    event_gk.S.Name' := args__c.(event_gk.S.Name');
+    event_gk.S.StartTime' := args__c.(event_gk.S.StartTime');
+    event_gk.S.EndTime' := args__c.(event_gk.S.EndTime')
+  |} with args__c; last (destruct args__c; reflexivity).
+  iApply "HΦ". iFrame.
 Qed.
 
 End Event_gk.
